rustfrontend/InitAnalysis.v
@@ -79,7 +79,7 @@ Local Open Scope error_monad_scope.
 
 (* The analyze returns the MaybeInit and MaybeUninit sets along with
 the universe set *)
-Definition analyze (ce: composite_env) (f: function) : Errors.res (PMap.t PathsMap.t * PMap.t PathsMap.t * PathsMap.t) :=
+Definition analyze (ce: composite_env) (f: function) (cfg: rustcfg) (entry: node) : Errors.res (PMap.t PathsMap.t * PMap.t PathsMap.t * PathsMap.t) :=
   (* collect the whole set in order to simplify the gen and kill operation *)
   do whole <- collect_func ce f;
   (* initialize maybeInit set with parameters *)
@@ -92,7 +92,7 @@ Definition analyze (ce: composite_env) (f: function) : Errors.res (PMap.t PathsM
   let vl := map (fun elt => Plocal (fst elt) (snd elt)) f.(fn_vars) in
   let maybeUninit := fold_right (add_place whole) empty_pathmap vl in
   (* generate selector-based CFG for analysis *)
-  do (entry, cfg) <- generate_cfg f.(fn_body);
+  (* do (entry, cfg) <- generate_cfg f.(fn_body); *)
   let initMap := DS.fixpoint cfg successors_instr (transfer whole true f cfg) entry maybeInit in
   let uninitMap := DS.fixpoint cfg successors_instr (transfer whole false f cfg) entry maybeUninit in
   match initMap, uninitMap with
@@ -153,9 +153,9 @@ Inductive tr_cont : statement -> rustcfg -> cont -> node -> option node -> optio
     (SEL: cfg ! loop_jump_node = Some (Inop body_start))
     (CONT: tr_cont body cfg k exit_loop cont brk nret),
     tr_cont body cfg (Kloop s k) loop_jump_node (Some loop_jump_node) (Some exit_loop) nret
-| tr_Kdropplace: forall body cfg k pc cont brk nret f st l le own
+| tr_Kdropplace: forall body cfg k pc cont brk nret f st l le own entry
     (CONT: tr_cont body cfg k pc cont brk nret)
-    (TRFUN: tr_fun f nret cfg),
+    (TRFUN: tr_fun f nret entry cfg),
     tr_cont body cfg (Kdropplace f st l le own k) pc cont brk nret
 | tr_Kdropcall: forall body cfg k pc cont brk nret st membs b ofs id
     (CONT: tr_cont body cfg k pc cont brk nret),
@@ -169,8 +169,8 @@ Inductive tr_cont : statement -> rustcfg -> cont -> node -> option node -> optio
 with tr_stacks: cont -> Prop :=
 | tr_stacks_stop:
   tr_stacks Kstop
-| tr_stacks_call: forall f nret cfg pc cont brk k own p le
-    (TRFUN: tr_fun f nret cfg)
+| tr_stacks_call: forall f nret cfg pc cont brk k own p le entry
+    (TRFUN: tr_fun f nret entry cfg)
     (TRCONT: tr_cont f.(fn_body) cfg k pc cont brk nret),
     tr_stacks (Kcall p f le own k).
 
@@ -226,7 +226,7 @@ Inductive sound_cont: cont -> Prop :=
     sound_cont k ->
     sound_cont (Kloop s k)
 | sound_cont_call: forall f initMap uninitMap pc mayinit mayuninit universe entry cfg k own1 own2 le p cont brk nret
-    (AN: analyze ce f = OK (initMap, uninitMap, universe))
+    (AN: analyze ce f cfg entry = OK (initMap, uninitMap, universe))
     (INIT: initMap !! pc = mayinit)
     (UNINIT: uninitMap !! pc = mayuninit)
     (CFG: generate_cfg f.(fn_body) = OK (entry, cfg))
@@ -238,11 +238,11 @@ Inductive sound_cont: cont -> Prop :=
     (OWN: sound_own own2 mayinit mayuninit universe)
     (CONT: sound_cont k),
     sound_cont (Kcall p f le own1 k)
-| sound_cont_dropplace: forall f initMap uninitMap pc mayinit mayuninit universe  cfg k own1 own2 le st l cont brk nret
-    (AN: analyze ce f = OK (initMap, uninitMap, universe))
+| sound_cont_dropplace: forall f initMap uninitMap pc mayinit mayuninit universe  cfg k own1 own2 le st l cont brk nret entry
+    (AN: analyze ce f cfg entry = OK (initMap, uninitMap, universe))
     (INIT: initMap !! pc =  mayinit)
     (UNINIT: uninitMap !! pc =  mayuninit)
-    (TRFUN: tr_fun f nret cfg)
+    (TRFUN: tr_fun f nret entry cfg)
     (TRCONT: tr_cont f.(fn_body) cfg k pc cont brk nret)
     (OWN: sound_own own2 mayinit mayuninit universe)
     (MOVESPLIT: move_split_places own1 l = own2)
@@ -255,12 +255,12 @@ Inductive sound_cont: cont -> Prop :=
 
   
 Inductive sound_state: state -> Prop :=
-| sound_regular_state: forall f initMap uninitMap pc mayinit mayuninit universe cfg s k own le m nret next cont brk
-    (AN: analyze ce f = OK (initMap, uninitMap, universe))
+| sound_regular_state: forall f initMap uninitMap pc mayinit mayuninit universe cfg s k own le m nret next cont brk entry
+    (AN: analyze ce f cfg entry = OK (initMap, uninitMap, universe))
     (INIT: initMap !! pc = mayinit)
     (UNINIT: uninitMap !! pc = mayuninit)
     (* invariant of generate_cfg *)
-    (TRFUN: tr_fun f nret cfg)
+    (TRFUN: tr_fun f nret entry cfg)
     (TRSTMT: tr_stmt f.(fn_body) cfg s pc next cont brk nret)
     (* k may be contain some statement not located in [next], e.g.,
     statements after continue and break *)
@@ -276,12 +276,12 @@ Inductive sound_state: state -> Prop :=
     (CONT: sound_cont k)
     (TRSTK: tr_stacks k),
     sound_state (Returnstate v k m)
-| sound_dropplace: forall f initMap uninitMap pc mayinit mayuninit universe cfg k own1 own2 le st l m nret cont brk
-    (AN: analyze ce f = OK (initMap, uninitMap, universe))
+| sound_dropplace: forall f initMap uninitMap pc mayinit mayuninit universe cfg k own1 own2 le st l m nret cont brk entry
+    (AN: analyze ce f cfg entry = OK (initMap, uninitMap, universe))
     (INIT: initMap !! pc = mayinit)
     (UNINIT: uninitMap !! pc = mayuninit)
     (* invariant of generate_cfg *)
-    (TRFUN: tr_fun f nret cfg)
+    (TRFUN: tr_fun f nret entry cfg)
     (TRCONT: tr_cont f.(fn_body) cfg k pc cont brk nret)
     (* small-step move_place to simulate big-step move_place in
     transfer. maybe difficult to prove *)
@@ -293,17 +293,10 @@ Inductive sound_state: state -> Prop :=
     (CONT: sound_cont k),
     sound_state (Dropstate id (Vptr b ofs) st membs k m)
 .
-
-(* inversion of analyze  *)
-Lemma analyze_function_inv: forall f initMap uninitMap universe
-    (AN: analyze ce f = OK (initMap, uninitMap, universe)),
-  exists entry cfg, generate_cfg f.(fn_body) = OK (entry, cfg).
-Admitted.
-
     
 (* soundness of function entry *)
 Lemma sound_function_entry: forall f initMap uninitMap universe entry cfg own
-    (AN: analyze ce f = OK (initMap, uninitMap, universe))
+    (AN: analyze ce f cfg entry = OK (initMap, uninitMap, universe))
     (CFG: generate_cfg f.(fn_body) = OK (entry, cfg))
     (FENTRY: init_own_env ce f = OK own),
     sound_own own initMap!!entry uninitMap!!entry universe.
@@ -332,11 +325,10 @@ Qed.
 (* use fixpoint_soulution to prove that the final abstract env
 approximates more than the abstract env computed by transfer
 function *)
-Lemma analyze_successor: forall f initMap uninitMap mayinit1 mayinit2 mayuninit1 mayuninit2 universe entry cfg instr pc1 pc2
-    (AN: analyze ce f = OK (initMap, uninitMap, universe))
+Lemma analyze_successor: forall f initMap uninitMap mayinit1 mayinit2 mayuninit1 mayuninit2 universe cfg entry instr pc1 pc2
+    (AN: analyze ce f cfg entry = OK (initMap, uninitMap, universe))
     (INIT: initMap !! pc1 = mayinit1)
     (UNINIT: uninitMap !! pc1 = mayuninit1)
-    (CFG: generate_cfg f.(fn_body) = OK (entry, cfg))
     (SEL: cfg ! pc1 = Some instr)
     (PC: In pc2 (successors_instr instr))
     (TFINIT: transfer universe true f cfg pc1 mayinit1 = mayinit2)
@@ -347,7 +339,6 @@ Lemma analyze_successor: forall f initMap uninitMap mayinit1 mayinit2 mayuninit1
 Proof.  (* use fixpoint_solution *)
   unfold analyze; intros. 
   Errors.monadInv AN.
-  rewrite EQ1 in CFG. inv CFG.
   set (params_init := (fold_right (add_place x)
                (PTree.map
                   (fun (_ : positive) (_ : LPaths.t) => Paths.empty) x)
@@ -363,7 +354,7 @@ Proof.  (* use fixpoint_solution *)
               params_init) eqn: INITMAP; try congruence.
   destruct (DS.fixpoint cfg successors_instr (transfer x false f cfg) entry
               vars_uninit) eqn: UNINITMAP; try congruence.
-  inv EQ2.
+  inv EQ0.
   split.
   - eapply DS.fixpoint_solution; eauto.
     (** TODO: transfer bot to bot *)
@@ -376,10 +367,9 @@ Admitted.
 (* use transfer to act as the bridge to construct the succ abstract
 env *)
 Lemma analyze_succ: forall f initMap uninitMap mayinit1 mayinit2 mayuninit1 mayuninit2 universe entry cfg instr own2 pc1 pc2
-    (AN: analyze ce f = OK (initMap, uninitMap, universe))
+    (AN: analyze ce f cfg entry = OK (initMap, uninitMap, universe))
     (INIT: initMap !! pc1 = mayinit1)
     (UNINIT: uninitMap !! pc1 = mayuninit1)
-    (CFG: generate_cfg f.(fn_body) = OK (entry, cfg))
     (SEL: cfg ! pc1 = Some instr)
     (PC: In pc2 (successors_instr instr))
     (TFINIT: transfer universe true f cfg pc1 mayinit1 = mayinit2)
@@ -406,13 +396,12 @@ Qed.
 
 
 Lemma sound_state_succ: forall f initMap uninitMap mayinit1 mayinit2 mayuninit1 mayuninit2 universe entry cfg instr1 own2 pc1 pc2 s k m le nret next cont brk
-    (AN: analyze ce f = OK (initMap, uninitMap, universe))
+    (AN: analyze ce f cfg entry = OK (initMap, uninitMap, universe))
     (INIT: initMap !! pc1 = mayinit1)
     (UNINIT: uninitMap !! pc1 = mayuninit1)
-    (CFG: generate_cfg f.(fn_body) = OK (entry, cfg))
     (SEL1: cfg ! pc1 = Some instr1)
     (PC: In pc2 (successors_instr instr1))
-    (TRFUN: tr_fun f nret cfg)
+    (TRFUN: tr_fun f nret entry cfg)
     (TRSTMT: tr_stmt f.(fn_body) cfg s pc2 next cont brk nret)
     (TRCONT: tr_cont f.(fn_body) cfg k next cont brk nret)
     (CONT: sound_cont k)
@@ -477,8 +466,9 @@ guaranteed by the compilation pass which actually uses the analyze
 function *)
 Hypothesis function_analyzed: forall (v : val) (f: function),
     Genv.find_funct ge v = Some (Internal f) ->
-    exists initMap uninitMap universe,
-      analyze ce f = OK (initMap, uninitMap, universe).
+    exists entry cfg nret initMap uninitMap universe,
+      tr_fun f nret entry cfg /\
+      analyze ce f cfg entry = OK (initMap, uninitMap, universe).
 
 
 Theorem sound_step: forall s t s',
@@ -552,7 +542,7 @@ Proof.
   - inv TRSTMT. econstructor.
     inv TRFUN.
     econstructor; eauto.
-    exploit analyze_succ. 1-4: eauto. eapply SEL.
+    exploit analyze_succ. 1-3: eauto. eapply SEL.
     instantiate (1 :=next). simpl. auto. eauto. eauto.
     (* prove sound_own *)
     instantiate (1 := move_place own2 p). admit.
@@ -560,26 +550,19 @@ Proof.
     econstructor; eauto.
   (* step_internal_function *)
   - exploit function_analyzed; eauto.
-    intros (initMap & uninitMap & universe & AN).
-    exploit analyze_function_inv; eauto.
-    intros (entry & cfg & CFG).
-    exploit generate_cfg_charact; eauto.
-    intros (nret & TRFUN).
+    intros (entry & cfg & nret & initMap & uninitMap & universe & TRFUN & AN).
+    inv TRFUN.
     inv ENTRY.
     exploit sound_function_entry; eauto.
     intros SOUND_INIT.
-    inv TRFUN. 
     econstructor; eauto.
     econstructor; eauto.
-    rewrite CFG in CFG0. inv CFG0. 
+    (* intros (nret & TRFUN). *)
     (* tr_cont *)
     inv TRSTK.
     econstructor. auto.
     econstructor; eauto.
     econstructor; eauto.
-    (* sound_own *)
-    rewrite CFG in CFG0. inv CFG0. 
-    auto.
   (* step_external_function *)    
   - econstructor; eauto.
   (* step_return_0 *)
@@ -596,6 +579,10 @@ Proof.
     eapply tr_stacks_call_cont; eauto.
   (* step_returnstate *)
   - inv TRSTK. inv CONT.
+    inv TRFUN.
+    rewrite CFG in CFG0. inv CFG0.
+    clear TRCONT0.
+    econstructor; eauto.         
     econstructor; eauto.
     econstructor.
     (* prove sound_own *)
@@ -632,7 +619,7 @@ Proof.
     econstructor; eauto.
     econstructor; eauto.
     inv TRFUN.
-    exploit analyze_succ. 1-4: eauto. eapply SEL.
+    exploit analyze_succ. 1-3: eauto. eapply SEL.
     simpl. eauto.
     unfold transfer. rewrite SEL. eauto.
     unfold transfer. rewrite SEL. eauto.
@@ -646,7 +633,7 @@ Proof.
     inv TRFUN.
     destruct H; inv H.
     + inv TRSTMT.
-      exploit analyze_succ. 1-4: eauto. eapply SEL.
+      exploit analyze_succ. 1-3: eauto. eapply SEL.
       simpl. eauto.
       unfold transfer. rewrite SEL. eauto.
       unfold transfer. rewrite SEL. eauto.
@@ -654,7 +641,7 @@ Proof.
       intros (mayinit3 & mayuninit3 & A & B & C).
       subst. auto.
     + inv TRSTMT.
-      exploit analyze_succ. 1-4: eauto. eapply SEL.
+      exploit analyze_succ. 1-3: eauto. eapply SEL.
       simpl. eauto.
       unfold transfer. rewrite SEL. eauto.
       unfold transfer. rewrite SEL. eauto.
